Update notation for atomic triples

atomic/weakestpre.v
@@ -12,23 +12,25 @@ example where we want it to be anything else. *)
 Definition atomic_wp `{!irisGS_gen hlc Λ Σ} {TA TB TC : tele}
   (e: expr Λ) (* expression *)
   (E : coPset) (* *implementation* mask *)
-  (α: TA → iProp Σ) (* atomic pre-condition *)
-  (β: TA → TB → iProp Σ) (* atomic post-condition *)
-  (Q: TA → TB → iProp Σ) (* private post-condition *)
+  (α: TA → iProp Σ) (* atomic precondition *)
+  (β: TA → TB → iProp Σ) (* atomic postcondition *)
+  (P: iProp Σ) (* private precondition *)
+  (Q: TA → TB → iProp Σ) (* private postcondition *)
   (Ψ: TC → iProp Σ)
   (f: TA → TB → val Λ) (* Turn the return data into the return value *)
   : iProp Σ :=
-    ∀ (Φ : val Λ → iProp Σ),
+    (□ ∀ (Φ : val Λ → iProp Σ),
+            P -∗
             (* The (outer) user mask is what is left after the implementation
             opened its things. *)
             atomic_update (⊤∖E) ∅ α Ψ β (λ.. x y, Q x y ={⊤∖E}=∗ Φ (f x y)) -∗
-            WP e {{ Φ }}.
+            WP e {{ Φ }})%I.
 (* Note: To add a private postcondition, use
    atomic_update α β Eo Ei (λ x y, POST x y -∗ Φ (f x y)) *)
 
 (* The way to read the [tele_app foo] here is that they convert the n-ary
 function [foo] into a unary function taking a telescope as the argument. *)
-Notation "'<<<' ∀∀ x1 .. xn , α '>>>' e @ E '<<<' ∃∃ y1 .. yn , β , 'RET' v '>>>' {{{ Q } } }" :=
+Notation "'<<<' ∀∀ x1 .. xn , α => ∃∃ y1 .. yn , β ; 'RET' v '>>>' @ E {{{ P } } } e {{{ Q } } }" :=
   (atomic_wp (TA:=TeleS (λ x1, .. (TeleS (λ xn, TeleO)) .. ))
              (TB:=TeleS (λ y1, .. (TeleS (λ yn, TeleO)) .. ))
              (TC:=TeleS (λ x1, .. (TeleS (λ xn, TeleO)) .. ))
@@ -38,6 +40,7 @@ Notation "'<<<' ∀∀ x1 .. xn , α '>>>' e @ E '<<<' ∃∃ y1 .. yn , β , 'R
              (tele_app $ λ x1, .. (λ xn,
                          tele_app (λ y1, .. (λ yn, β%I) .. )
                         ) .. )
+             P
              (tele_app $ λ x1, .. (λ xn,
                          tele_app (λ y1, .. (λ yn, Q%I) .. )
                         ) .. )
@@ -46,11 +49,11 @@ Notation "'<<<' ∀∀ x1 .. xn , α '>>>' e @ E '<<<' ∃∃ y1 .. yn , β , 'R
                          tele_app (λ y1, .. (λ yn, v%V) .. )
                         ) .. )
   )
-  (at level 20, E, α, β, Q, v at level 200, x1 binder, xn binder, y1 binder, yn binder,
-   format "'[hv' '<<<'  '[' ∀∀  x1  ..  xn ,  '/' α  ']' '>>>'  '/  ' e  @  E  '/' '<<<'  '[' ∃∃  y1  ..  yn ,  '/' β ,  '/' 'RET'  v  ']' '>>>' {{{ '[' Q ']' } } } ']'")
+  (at level 20, E, α, β, P, Q, v at level 200, x1 binder, xn binder, y1 binder, yn binder,
+   format "'[hv' '<<<' '[' ∀∀ x1 .. xn , α => ∃∃ y1 .. yn , β ; 'RET' v ']' '>>>' @ E {{{ '[' P ']' } } } e {{{ '[' Q ']' } } } ']'")
   : bi_scope.
 
-Notation "'<<<' ∀∀ x1 .. xn , α '>>>' e @ E '<<<' β , 'RET' v '>>>' {{{ Q } } }" :=
+Notation "'<<<' ∀∀ x1 .. xn , α => β ; 'RET' v '>>>' @ E {{{ P } } } e {{{ Q } } }" :=
   (atomic_wp (TA:=TeleS (λ x1, .. (TeleS (λ xn, TeleO)) .. ))
              (TB:=TeleO)
              (TC:=TeleS (λ x1, .. (TeleS (λ xn, TeleO)) .. ))
@@ -58,15 +61,16 @@ Notation "'<<<' ∀∀ x1 .. xn , α '>>>' e @ E '<<<' β , 'RET' v '>>>' {{{ Q 
              E
              (tele_app $ λ x1, .. (λ xn, α%I) ..)
              (tele_app $ λ x1, .. (λ xn, tele_app β%I) .. )
+             P
              (tele_app $ λ x1, .. (λ xn, tele_app Q%I) .. )
              (tele_app $ λ x1, .. (λ xn, α%I) ..)
              (tele_app $ λ x1, .. (λ xn, tele_app v%V) .. )
   )
-  (at level 20, E, α, β, Q, v at level 200, x1 binder, xn binder,
-   format "'[hv' '<<<'  '[' ∀∀  x1  ..  xn ,  '/' α  ']' '>>>'  '/  ' e  @  E  '/' '<<<'  '[' β ,  '/' 'RET'  v  ']' '>>>' {{{ '[' Q ']' } } } ']'")
+  (at level 20, E, α, β, P, Q, v at level 200, x1 binder, xn binder,
+   format "'[hv' '<<<' '[' ∀∀ x1 .. xn , α => β ; 'RET' v ']' '>>>' @ E {{{ '[' P ']' } } } e {{{ '[' Q ']' } } } ']'")
   : bi_scope.
 
-Notation "'<<<' α '>>>' e @ E '<<<' ∃∃ y1 .. yn , β , 'RET' v '>>>' {{{ Q } } }" :=
+Notation "'<<<' α => ∃∃ y1 .. yn , β ; 'RET' v '>>>' @ E {{{ P } } } e {{{ Q } } }" :=
   (atomic_wp (TA:=TeleO)
              (TB:=TeleS (λ y1, .. (TeleS (λ yn, TeleO)) .. ))
              (TC:=TeleO)
@@ -74,15 +78,16 @@ Notation "'<<<' α '>>>' e @ E '<<<' ∃∃ y1 .. yn , β , 'RET' v '>>>' {{{ Q 
              E
              (tele_app α%I)
              (tele_app $ tele_app (λ y1, .. (λ yn, β%I) .. ))
+             P
              (tele_app $ tele_app (λ y1, .. (λ yn, Q%I) .. ))
              (tele_app α%I)
              (tele_app $ tele_app (λ y1, .. (λ yn, v%V) .. ))
   )
-  (at level 20, E, α, β, Q, v at level 200, y1 binder, yn binder,
-   format "'[hv' '<<<'  '[' α  ']' '>>>'  '/  ' e  @  E  '/' '<<<'  '[' ∃∃  y1  ..  yn ,  '/' β ,  '/' 'RET'  v  ']' '>>>' {{{ '[' Q ']' } } } ']'")
+  (at level 20, E, α, β, P, Q, v at level 200, y1 binder, yn binder,
+   format "'[hv' '<<<' '[' α => ∃∃ y1 .. yn , β ; 'RET' v ']' '>>>' @ E {{{ '[' P ']' } } } e {{{ '[' Q ']' } } } ']'")
   : bi_scope.
 
-Notation "'<<<' α '>>>' e @ E '<<<' β , 'RET' v '>>>' {{{ Q } } }" :=
+Notation "'<<<' α => β ; 'RET' v '>>>' @ E {{{ P } } } e {{{ Q } } }" :=
   (atomic_wp (TA:=TeleO)
              (TB:=TeleO)
              (TC:=TeleO)
@@ -90,12 +95,13 @@ Notation "'<<<' α '>>>' e @ E '<<<' β , 'RET' v '>>>' {{{ Q } } }" :=
              E
              (tele_app α%I)
              (tele_app $ tele_app β%I)
+             P
              (tele_app $ tele_app Q%I)
              (tele_app α%I)
              (tele_app $ tele_app v%V)
   )
-  (at level 20, E, α, β, Q, v at level 200,
-   format "'[hv' '<<<'  '[' α  ']' '>>>'  '/  ' e  @  E  '/' '<<<'  '[' β ,  '/' 'RET'  v  ']' '>>>' {{{ '[' Q ']' } } } ']'")
+  (at level 20, E, α, β, P, Q, v at level 200,
+   format "'[hv' '<<<' '[' α => β ; 'RET' v ']' '>>>' @ E {{{ '[' P ']' } } } e {{{ '[' Q ']' } } } ']'")
   : bi_scope.
 
 (** Theory *)
@@ -105,15 +111,16 @@ Section lemmas.
   Implicit Types (α : TA → iProp) (β Q : TA → TB → iProp) (Ψ : TC → iProp) (f : TA → TB → val Λ).
 
   (* Atomic triples imply sequential triples. *)
-  Lemma atomic_wp_seq e E α β Q Ψ f :
-    atomic_wp e E α β Q Ψ f -∗
-    ∀ Φ, ∀.. x, α x -∗
+  Lemma atomic_wp_seq e E α β P Q Ψ f :
+    atomic_wp e E α β P Q Ψ f -∗
+    ∀ Φ, P -∗
+    ∀.. x, α x -∗
     (∀.. y, β x y -∗ (Q x y -∗ Φ (f x y))) -∗
     (∀.. y, β x y -∗ ∃.. z, Ψ z ∗ (Ψ z -∗ β x y)) -∗
     WP e {{ Φ }}.
   Proof.
-    iIntros "Hwp" (Φ x) "Hα HΦ HΨ".
-    iApply (wp_frame_wand with "HΦ"). iApply "Hwp".
+    iIntros "Hwp %Φ HP %x Hα HΦ HΨ".
+    iApply (wp_frame_wand with "HΦ"). iApply ("Hwp" with "HP").
     iAuIntro. iAaccIntro with "Hα". 
     { iIntros; iModIntro; iFrame. }
     iIntros (y) "Hβ !>".
@@ -126,29 +133,30 @@ Section lemmas.
 
   (** This version matches the Texan triple, i.e., with a later in front of the
   [(∀.. y, β x y -∗ Φ (f x y))]. *)
-  Lemma atomic_wp_seq_step e E α β Q Ψ f :
+  Lemma atomic_wp_seq_step e E α β P Q Ψ f :
     TCEq (to_val e) None →
-    atomic_wp e E α β Q Ψ f -∗
-    ∀ Φ, ∀.. x, α x -∗
+    atomic_wp e E α β P Q Ψ f -∗
+    ∀ Φ, P -∗
+    ∀.. x, α x -∗
     ▷ (∀.. y, β x y -∗ (Q x y -∗ Φ (f x y))) -∗
     (∀.. y, β x y -∗ ∃.. z, Ψ z ∗ (Ψ z -∗ β x y)) -∗
     WP e {{ Φ }}.
   Proof.
-    iIntros (?) "H"; iIntros (Φ x) "Hα HΦ HΨ".
+    iIntros (?) "Hwp %Φ HP %x Hα HΦ HΨ".
     iApply (wp_step_fupd _ _ ⊤ _ (∀.. y, β x y -∗ (Q x y -∗ Φ (f x y)))
       with "[$HΦ //]"); first done.
-    iApply (atomic_wp_seq with "H Hα [] HΨ").
+    iApply (atomic_wp_seq with "Hwp HP Hα [] HΨ").
     iIntros (y) "Hβ HQ HΦ". iModIntro.
     iApply ("HΦ" with "Hβ HQ").
   Qed.
 
   (* Sequential triples with the empty mask for a physically atomic [e] are atomic. *)
-  Lemma atomic_seq_wp_atomic e E α β Q Ψ f `{!Atomic WeaklyAtomic e} :
-    (∀ Φ, ∀.. x, α x -∗ (∀.. y, β x y -∗ (Q x y -∗ Φ (f x y))) -∗ WP e @ ∅ {{ Φ }}) -∗
-    atomic_wp e E α β Q Ψ f.
+  Lemma atomic_seq_wp_atomic e E α β P Q Ψ f `{!Atomic WeaklyAtomic e} :
+    (□ ∀ Φ, P -∗ ∀.. x, α x -∗ (∀.. y, β x y -∗ (Q x y -∗ Φ (f x y))) -∗ WP e @ ∅ {{ Φ }}) -∗
+    atomic_wp e E α β P Q Ψ f.
   Proof.
-    iIntros "Hwp" (Φ) "AU". iMod "AU" as (x) "[Hα [_ Hclose]]".
-    iApply ("Hwp" with "Hα"). iIntros (y) "Hβ HQ".
+    iIntros "#Hwp %Φ !> HP AU". iMod "AU" as (x) "[Hα [_ Hclose]]".
+    iApply ("Hwp" with "HP Hα"). iIntros (y) "Hβ HQ".
     iMod ("Hclose" with "Hβ") as "AP". rewrite ->!tele_app_bind. 
     iMod "AP" as (z) "[HΨ [_ HΦ]]". iMod ("HΦ" with "HΨ") as "HΦ".
     iDestruct ("HΦ" with "HQ") as "HΦ".
@@ -159,16 +167,16 @@ Section lemmas.
   (** Sequential triples with a persistent precondition and no initial quantifier
   are atomic. *)
   Lemma persistent_seq_wp_atomic e E (α : [tele] → iProp) 
-        (β : [tele] → TB → iProp) (Q : [tele] → TB → iProp) Ψ
+        (β : [tele] → TB → iProp) (P : iProp) (Q : [tele] → TB → iProp) Ψ
         (f : [tele] → TB → val Λ) {HP : Persistent (α [tele_arg])} :
-    (∀ Φ, α [tele_arg] -∗ 
+    (□ ∀ Φ, P -∗ α [tele_arg] -∗ 
       (∀.. y, β [tele_arg] y -∗ (Q [tele_arg] y -∗ Φ (f [tele_arg] y))) -∗ WP e {{ Φ }}
     ) -∗
-    atomic_wp e E α β Q Ψ f.
+    atomic_wp e E α β P Q Ψ f.
   Proof.
-    simpl in HP. iIntros "Hwp" (Φ) "HΦ". iApply fupd_wp.
-    iMod ("HΦ") as "[#Hα [Hclose _]]". iMod ("Hclose" with "Hα") as "HΦ".
-    iApply wp_fupd. iApply ("Hwp" with "Hα"). iIntros "!>" (y) "Hβ HQ".
+    simpl in HP. iIntros "#Hwp %Φ !> HP AU ". iApply fupd_wp.
+    iMod ("AU") as "[#Hα [Hclose _]]". iMod ("Hclose" with "Hα") as "HΦ".
+    iModIntro. iApply wp_fupd. iApply ("Hwp" with "HP Hα"). iIntros (y) "Hβ HQ".
     iMod ("HΦ") as "[_ [_ Hclose]]". iMod ("Hclose" with "Hβ") as "HΦ".
     rewrite ->!tele_app_bind. iMod "HΦ" as (z) "[HΨ [_ HΦ]]".
     iMod ("HΦ" with "HΨ") as "HΦ". iDestruct ("HΦ" with "HQ") as "HΦ".
@@ -176,10 +184,10 @@ Section lemmas.
     solve_ndisj.
   Qed.
 
-  Lemma atomic_wp_mask_weaken e E1 E2 α β Q Ψ f :
-    E1 ⊆ E2 → atomic_wp e E1 α β Q Ψ f -∗ atomic_wp e E2 α β Q Ψ f.
+  Lemma atomic_wp_mask_weaken e E1 E2 α β P Q Ψ f :
+    E1 ⊆ E2 → atomic_wp e E1 α β P Q Ψ f -∗ atomic_wp e E2 α β P Q Ψ f.
   Proof.
-    iIntros (HE) "Hwp". iIntros (Φ) "AU". iApply "Hwp".
+    iIntros (HE) "#Hwp !> %Φ HP AU". iApply ("Hwp" with "HP").
     iApply (atomic_update_mask_weaken (⊤ ∖ E2)); first solve_ndisj.
     iApply (atomic_update_wand with "[] AU").
     iIntros (x y) "HΦ". rewrite ->!tele_app_bind.
@@ -190,22 +198,22 @@ Section lemmas.
 
   (** We can open invariants around atomic triples.
       (Just for demonstration purposes; we always use [iInv] in proofs.) *)
-  Lemma atomic_wp_inv e E α β Q f N I :
+  Lemma atomic_wp_inv e E α β P Q f N I :
     ↑N ⊆ E →
-    atomic_wp e (E ∖ ↑N) (λ.. x, ▷ I ∗ α x) (λ.. x y, ▷ I ∗ β x y) Q (λ.. x, ▷ I ∗ α x) f -∗
-    inv N I -∗ atomic_wp e E α β Q α f.
+    atomic_wp e (E ∖ ↑N) (λ.. x, ▷ I ∗ α x) (λ.. x y, ▷ I ∗ β x y) P Q (λ.. x, ▷ I ∗ α x) f -∗
+    inv N I -∗ atomic_wp e E α β P Q α f.
   Proof.
-    iIntros "%HE Hwp #Hinv" (Φ) "AU". iApply "Hwp".
+    iIntros "%HE #Hwp #Hinv !> %Φ HP AU". iApply ("Hwp" with "HP").
     replace (⊤ ∖ E) with (⊤ ∖ (E ∖ ↑N) ∖ ↑N) by set_solver.
     iApply (aupd_inv with "Hinv AU"); solve_ndisj.
   Qed.
 
-  Lemma atomic_wp_inv_timeless e E α β Q f N I `{!Timeless I} :
+  Lemma atomic_wp_inv_timeless e E α β P Q f N I `{!Timeless I} :
     ↑N ⊆ E →
-    atomic_wp e (E ∖ ↑N) (λ.. x, I ∗ α x) (λ.. x y, I ∗ β x y) Q (λ.. x, I ∗ α x) f -∗
-    inv N I -∗ atomic_wp e E α β Q α f.
+    atomic_wp e (E ∖ ↑N) (λ.. x, I ∗ α x) (λ.. x y, I ∗ β x y) P Q (λ.. x, I ∗ α x) f -∗
+    inv N I -∗ atomic_wp e E α β P Q α f.
   Proof.
-    iIntros "%HE Hwp #Hinv" (Φ) "AU". iApply "Hwp".
+    iIntros "%HE #Hwp #Hinv !> %Φ HP AU". iApply ("Hwp" with "HP").
     replace (⊤ ∖ E) with (⊤ ∖ (E ∖ ↑N) ∖ ↑N) by set_solver.
     iApply (aupd_inv_timeless with "Hinv AU"); solve_ndisj.
   Qed.
