lazy_list/spec/find.v
@@ -16,14 +16,14 @@ Module FindSpec (Params: LAZY_LIST_PARAMS).
 
     Theorem find_spec (k: Z) (head curr: node_rep) (Γ: lazy_gname) :
       node_key curr < k < INT_MAX →
-      (⌜ curr = head ⌝ ∨ own Γ.(auth_gname) (◯ {[curr]})) -∗
-      <<< ∀∀ (S: gset node_rep), lazy_list head S Γ >>>
-        find (rep_to_node curr) #k @ ∅
-      <<< ∃∃ pred succ, 
-        lazy_list head S Γ
-        ∗
-        ⌜ k = node_key succ ↔ k ∈ (set_map node_key S : gset Z) ⌝, 
-      RET ((rep_to_node pred), (rep_to_node succ)) >>>
+      ⊢ <<< 
+        ∀∀ (S: gset node_rep), lazy_list head S Γ =>
+        ∃∃ pred succ, lazy_list head S Γ ∗ 
+          ⌜ k = node_key succ ↔ k ∈ (set_map node_key S : gset Z) ⌝; 
+        RET ((rep_to_node pred), (rep_to_node succ))
+      >>> @ ∅
+      {{{ ⌜ curr = head ⌝ ∨ own Γ.(auth_gname) (◯ {[curr]}) }}}
+        find (rep_to_node curr) #k
       {{{ 
         (⌜ pred = head ⌝ ∨ own Γ.(auth_gname) (◯ {[pred]}))
         ∗
@@ -32,7 +32,7 @@ Module FindSpec (Params: LAZY_LIST_PARAMS).
         ⌜ node_key pred < k ≤ node_key succ ⌝
       }}}.
     Proof.
-      iIntros "%Hk Hcurr %Φ"; iRevert (curr Hk) "Hcurr".
+      iIntros "%Hk !> %Φ Hcurr"; iRevert (curr Hk) "Hcurr".
       iLöb as "IH"; iIntros (curr Hk) "#Hcurr AU".
       rewrite difference_empty_L.
       wp_lam. wp_let. wp_lam. wp_pures.
@@ -70,14 +70,14 @@ Module FindSpec (Params: LAZY_LIST_PARAMS).
 
     Theorem findLock_spec (k: Z) (head curr: node_rep) (Γ: lazy_gname) :
       node_key curr < k < INT_MAX →
-      (⌜ curr = head ⌝ ∨ own Γ.(auth_gname) (◯ {[curr]})) -∗
-      <<< ∀∀ (S: gset node_rep), lazy_list head S Γ >>>
-        findLock (rep_to_node curr) #k @ ∅
-      <<< ∃∃ pred succ,
-        lazy_list head S Γ
-        ∗
-        ⌜ k = node_key succ ↔ k ∈ (set_map node_key S : gset Z) ⌝,
-      RET ((rep_to_node pred), (rep_to_node succ)) >>>
+      ⊢ <<< 
+        ∀∀ (S: gset node_rep), lazy_list head S Γ =>
+        ∃∃ pred succ, lazy_list head S Γ ∗
+          ⌜ k = node_key succ ↔ k ∈ (set_map node_key S : gset Z) ⌝;
+        RET ((rep_to_node pred), (rep_to_node succ))
+      >>> @ ∅
+      {{{ ⌜ curr = head ⌝ ∨ own Γ.(auth_gname) (◯ {[curr]}) }}}
+        findLock (rep_to_node curr) #k
       {{{
         (⌜ pred = head ⌝ ∨ own Γ.(auth_gname) (◯ {[pred]}))
         ∗
@@ -90,7 +90,7 @@ Module FindSpec (Params: LAZY_LIST_PARAMS).
         acquired #(node_lock pred)
       }}}.
     Proof.
-      iIntros "%Hk Hcurr %Φ"; iRevert (curr Hk) "Hcurr".
+      iIntros "%Hk !> %Φ Hcurr"; iRevert (curr Hk) "Hcurr".
       iLöb as "IH"; iIntros (curr Hk) "#Hcurr AU".
       rewrite difference_empty_L.
       wp_lam. wp_let.
@@ -105,7 +105,7 @@ Module FindSpec (Params: LAZY_LIST_PARAMS).
       iModIntro. iIntros "(#Hpred & _ & [%Hk' _])".
       iModIntro. wp_pures; wp_lam; wp_pures.
 
-      awp_apply acquire_spec.
+      awp_apply (acquire_spec with "[$]").
       iApply (aacc_aupd_sub with "[] AU"); try done.
       { 
         iIntros "!> %S H". iDestruct (lazy_node_has_lock with "Hpred H") as "[Hlock Hlazy]".
